---
layout: post
title: 테스트 $p\sum_{k=0}^{\infty}{q^k} = p\frac{\partial}{\partial q}\left( \sum_{k=1}^{\infty}{q^k} \right) = p\sum_{k=1}^{\infty}kq^{k-1} $
author: piorosen
categories: [Blogging, Develop]
tags: [deep-learning,compiler,survey,paper,review,xla,tvm]
hide_title: false
math: true
---


$p\sum_{k=0}^{\infty}{q^k} = p\frac{\partial}{\partial q}\left( \sum_{k=1}^{\infty}{q^k} \right) = p\sum_{k=1}^{\infty}kq^{k-1} $

# $p\sum_{k=0}^{\infty}{q^k} = p\frac{\partial}{\partial q}\left( \sum_{k=1}^{\infty}{q^k} \right) = p\sum_{k=1}^{\infty}kq^{k-1} $
